[WIP]

theories/l2t.v
@@ -124,17 +124,32 @@ Proof.
   - move=> s bt []//[]// s1 []// []//= [|[]]//=[]//[|[]]//; case: bt => //=.
 Abort.
 
-Definition add_ca_deep_lvl1 (bt:alts) (a: alts) : alts := 
-  map (fun '(s,xs) => (s,map (apply_cut (fun ca => add_ca_deep bt ca)) xs)) a.
+(* Definition add_ca_deep_lvl1 (bt:alts) (a: alts) : alts := 
+  map (fun '(s,xs) => (s,map (apply_cut (fun ca => add_ca_deep bt ca)) xs)) a. *)
 
-Lemma split_cat {x1 x2: alts} {F r}:
+(* Lemma split_cat {x1 x2: alts} {F r}:
   x1 ++ x2 = map F r -> Texists p1 p2, p1 ++ p2 = r /\ x1 = map F p1 /\ x2 = map F p2.
 Proof.
-Admitted.
+Admitted. *)
+
+(* Lemma s2l_add_ca {A s xs}:
+  state_to_list A s nilC = add_ca_deep nilC xs ->
+    forall bt2, state_to_list A s bt2 = add_ca_deep bt2 xs.
+Proof.
+  elim: A s xs => //=.
+  - move=> _ []//.
+  - move=> []//.
+  - move=> s []//[]//s1 []//[]//=[]s2 []//.
+  - move=> s []//=[]s1[]//[]//=[]s2[]//=.
+  - move=> _ []//[]//.
+  - move=> p c s1 []//[s2][]//[]//p1 c1 []//[]//=[s3]//.
+  - move=> s []//[]s1[]//[]//=a.
+    rewrite add_ca_deep_empty1.
+    case: a => //-[]//=[|[]]//. *)
 
 (* Lemma s2l_add_ca {A s xs bt1}:
-  state_to_list A s bt1 = add_ca_deep_lvl1 bt1 xs ->
-    forall bt2, state_to_list A s bt2 = add_ca_deep_lvl1 bt2 xs.
+  state_to_list A s bt1 = add_ca_deep bt1 xs ->
+    forall bt2, state_to_list A s bt2 = add_ca_deep bt2 xs.
 Proof.
   (* rewrite /add_ca_deep_lvl1. *)
   elim: A s xs bt1 => //=.
@@ -157,7 +172,17 @@ Proof.
 
 Abort. *)
 
-Lemma xx {u A s s1 bt xs}:
+(* Fixpoint describe_nilC A :=
+  match A with
+  | Or A _ B =>
+    if is_ko A then describe_nilC B
+    else describe_nilC A
+  | And A _ B => describe_nilC A && describe_nilC B
+  | Top | OK => true
+  | CallS _ _ | CutS | Dead | Bot => false
+  end. *)
+
+Lemma valid_state_nil_run {u A s s1 bt xs}:
   valid_state A ->
   state_to_list A s bt = (s1, nilC) ::: xs ->
   Texists B n,
@@ -236,24 +261,162 @@ Proof.
     admit. (*this is ok: A /\ B with run A and run B and B0 = B*)
 Admitted.
 
-Search runb And.
-    
+Lemma add_ca_deep_inj {bt a1 a2}:  
+  add_ca_deep bt a1 = add_ca_deep bt a2 -> a1 = a2
+with add_ca_deep_goals_inj {bt g1 g2}:
+  add_ca_deep_goals bt g1 = add_ca_deep_goals bt g2 -> g1 = g2
+with add_ca_deep_g_inj {bt g1 g2}:
+  add_ca_deep_g bt g1 = add_ca_deep_g bt g2 -> g1 = g2.
+Proof.
+  - case: a1 => [|[]].
+      case: a2 => [|[]]//.
+    case: a2 => [|[]]//s1 x xs s2 y ys[?] /add_ca_deep_goals_inj ? /add_ca_deep_inj ?; by subst.
+  - case: g1; case: g2 => //= x xs y ys []/add_ca_deep_g_inj? /add_ca_deep_goals_inj?; by subst.
+  - by case: g1; case: g2 => //xs ys [] /append_sameR /add_ca_deep_inj->.
+Qed.
 
-Lemma two' {u s s1} {alts alts_left : alts} {andg : goals}  : 
-  nur u s andg alts s1 alts_left -> forall t bt,
+(* HYP: A is not failed *)
+Fixpoint next_cut (A: state) :=
+  match A with
+  | Or A s B =>
+    (* HERE THE PROBLEM: should not next_cut on is_ko but on is_dead A *)
+    if is_ko A then (false, Or (if is_dead A then A else dead1 A) s (next_cut B).2)
+    else 
+      let '(b1, A') := next_cut A in
+      (false, Or A' s (if b1 then cutr B else B))
+  | And A B0 B =>
+    if success A then
+      let '(c, B') := next_cut B in
+      (c, And (if c then cutl A else A) (if c then cutl B0 else B0) B')
+    else
+    let '(b1, A') := next_cut A in
+    (b1, And A' B0 B)
+  | CutS => (true, OK)
+  | Top | OK | CallS _ _ | Dead | Bot => (false, A)
+  end.
+
+Lemma next_cut_success {A B}: success A -> next_cut A = B -> success B.2.
+Proof.
+  move=> + <- {B}; elim: A => //=.
+  - move=> A HA s B HB; case: ifP => [dA sB|dA sA].
+      rewrite is_dead_is_ko//=dA HB//.
+    rewrite success_is_ko//.
+    move: HA; case: next_cut => //=b A' /(_ sA) sA'.
+    rewrite success_is_dead//.
+  - move=> A + B0 _ B + /andP[sA sB] => - /(_ sA) + /(_ sB).
+    case: next_cut => //=b A' sA'.
+    rewrite sA.
+    case: next_cut => //=b' B' ->.
+    by rewrite fun_if success_cut sA if_same.
+Qed.
+
+Lemma next_alt_is_and {A B}:
+  is_and A -> next_cut A = B -> is_and B.2.
+Proof.
+  move=> + <- {B}; elim: A => //-[]//=.
+  - move=> _ B HB C HC /HC; case: next_cut => //= a b; rewrite if_same//.
+  - move=> A s B _ C HC D HD /[dup] aD /HD; case: next_cut => //= b E aE.
+    (repeat case: ifP => //=).
+      case: next_cut => //=b' F; case: ifP => //.
+    case: next_cut => //=b' F; case: ifP => //.
+  - move=> A B0 B _ C HC D HD/[dup] aD /HD.
+    case: next_cut => //= b E.
+    case: next_cut => //=??.
+    case: next_cut => //=??.
+    repeat case: ifP => //=.
+Qed.
+
+Lemma next_alt_is_or {A B}:
+  is_or A -> next_cut A = B -> is_or B.2.
+Proof.
+  move=> + <- {B}; elim: A => //-[]//=.
+  - move=> A s B _ C s1 D _.
+    repeat case: ifP => //.
+    case: next_cut => //.
+  - move=> A B0 B _ s1 D HD _.
+    repeat case: ifP => //.
+    case: next_cut => // ???.
+    case: next_cut => //.
+Qed.
+
+Lemma next_cut_valid {A B}: 
+  failed A = false -> valid_state A -> next_cut A = B -> valid_state B.2.
+Proof.
+  move=> ++ <-; clear B.
+  elim: A => //=.
+  - move=> A HA s B HB.
+    case: ifP => [dA fB vB|dA fA /andP[vA bB]].
+      by rewrite is_dead_is_ko//=dA HB.
+    case: ifP => kA/=.
+      by rewrite is_ko_failed in fA.
+    move: (HA fA vA).
+    case X: next_cut => [b A']/= vA'.
+    rewrite valid_state_dead1//=vA'.
+    case: ifP; rewrite//= bbOr_cutr//.
+  - move=> A HA B0 _ B HB + /and5P[oA vA aA].
+    case fA: failed => //=.
+    case: ifP => /=[sA fB vB bB|sA _ /eqP->{B0}].
+      move: (HA fA vA) (HB fB vB) => {HA HB}.
+      case X: next_cut => //= [b A'].
+      case Y: next_cut => //= [b' B'] vA' vB'.
+      rewrite (fun_if success) success_cut if_same.
+      have sA' := next_cut_success sA X.
+      rewrite (fun_if is_or) (fun_if valid_state) (fun_if bbAnd)/=.
+      rewrite valid_state_cut// vB'.
+      rewrite (next_alt_is_and aA Y) bB /bbAnd bbAnd_cutl// orbT.
+      have /= oA' := next_alt_is_or oA X.
+      by rewrite is_or_cutl//sA/=vA oA if_same//.
+    move=> bB.
+    have {HB} :=  HB (base_and_failed bB) (base_and_valid bB).
+    have {HA} :=  HA fA vA.
+    case X: next_cut => //= [bA A'].
+    case Y: next_cut => //= [b' B'] vA' vB'.
+    have /= oA':= next_alt_is_or oA X.
+    have /= aB':= next_alt_is_and aA Y.
+    by rewrite vA' oA' base_and_is_and// eqxx base_and_valid///bbAnd bB !if_same.
+Qed.
+
+Lemma next_cut_s2l {b A A' s bt s1 ca gl a}:
+  failed A = false -> state_to_list A s bt = 
+     (s1, (cut (add_ca_deep bt ca ++ bt)) ::: (add_ca_deep_goals bt gl)) ::: (add_ca_deep bt a) ->
+    next_cut A = (b, A') ->
+      state_to_list A' s bt = add_ca_deep bt (s1, gl) ::: ca.
+Proof.
+Admitted.
+
+Lemma two' {u s1 s2} {alts alts_left : alts} {andg : goals}  : 
+  nur u s1 andg alts s2 alts_left -> forall s t bt,
   valid_state t ->
-  state_to_list t s bt = add_ca_deep bt ((s,andg) ::: alts) -> 
+  (* TODO: not sure the following equation is valid *)
+  state_to_list t s bt = add_ca_deep bt ((s1,andg) ::: alts) -> 
   Texists t1 n,
-    runb u s t s1 t1 n
+    runb u s t s2 t1 n
       (* /\ state_to_list (odflt Bot t1) s1 bt1 = add_ca_deep bt1 alts_left  *)
     .
 Proof.
   elim; clear.
-
-  - move=> s a t bt1 /= vt Ht.
-    apply: xx vt Ht.
-  - move=> s1 s2 a ca r gl H IH t bt H1.
-    admit.
+  - move=> s a t s1 bt1 /= vt Ht.
+    apply: valid_state_nil_run vt Ht.
+    {
+      move=> s1 s2 a ca r gl ELPI IH s A bt vA H.
+      (* TODO: should induction until the state is not failed *)
+      (* if it is failed, it is equivalent to apply n times run_fail on the conclusion *)
+      (* TODO: should apply run_fail till failed A = true, then we apply IH *)
+      (* therefore the state we pass to IH is not failed *)
+        case X: (next_cut A) => [b A'].
+        (* add_ca_deep bt (s1, (cut ca) ::: gl) ::: a *)
+        (* add_ca_deep bt (s1, gl) ::: ca *)
+        simpl in H.
+        have H1 := next_cut_s2l _ H X.
+        have {} := IH _ A' _ (next_cut_valid _ vA X) (H1 _).
+        case fA: (failed A); last first.
+        case: b X => X /(_ erefl erefl) [A''[n {}IH]].
+          repeat eexists; apply: run_cut _ IH.
+          admit.
+        repeat eexists; apply: run_step _ IH.
+        admit.
+      admit.
+    }
   - admit.
   - admit.
 Admitted.
