theories/elpi.v
@@ -185,6 +185,7 @@ Class IsList {Th Tl : Type}  := {
   map_cons F l1 l2 : map F (consC l1 l2) = consC (F l1) (map F l2);
   size_map F l1 : size (map F l1) = size l1;
   map_id l1 : map id l1 = l1;
+  append_sameR {l1 l2 l3}: appendC l1 l3 = appendC l2 l3 -> l1 = l2; 
 }.
 Declare Scope SE.
 Global Infix "++" := appendC : SE.
@@ -460,6 +461,10 @@ Section alts.
     move=> F l1; elim: l1 => //=x xs IH l1; rewrite IH//.
     move=> F l1; elim: l1 => //=_ xs->//.
     move=>l; elim: l => //=g gs->//.
+    elim => [|[s g] gs IH] [|[s1 g1] gs1]//= l3.
+      + move=> /(f_equal size_alts)/=; rewrite size_cat_alts; lia.
+      + move=> /(f_equal size_alts)/=; rewrite size_cat_alts; lia.
+      + by move=> [??]/IH?; subst.
   Defined.
 End alts.
 
@@ -602,6 +607,10 @@ Section goals.
     move=> F l1; elim: l1 => //=x xs IH l1; rewrite IH//.
     move=> F l1; elim: l1 => //=_ xs->//.
     move=> l; elim: l => //=x xs->//.
+    elim => [|g gs IH] [|g1 gs1]//= l3.
+      + move=> /(f_equal size_goals)/=; rewrite size_cat_goals; lia.
+      + move=> /(f_equal size_goals)/=; rewrite size_cat_goals; lia.
+      + by move=> [?]/IH?; subst.
   Defined.
 End goals.
 
